prog0/lambda-formalizations/LambdaEnv.lean
@@ -1,1 +1,2 @@
 import LambdaEnv.Syntax
+import LambdaEnv.Reduction
